État du dépôt à la fin de la visite.

src/HLPL_plus.v
@@ -1,20 +1,22 @@
 Require Import base.
 Require Import PathToSubtree.
 Require Import lang.
+Require Import List.
+Import ListNotations.
 
 Variant HLPL_plus_zero :=
 | HLPL_plus_bot
 | HLPL_plus_int (n : nat) (* TODO: use Aeneas integer types? *)
-| HLPL_plus_loan (l : loc)
-| HLPL_plus_ptr (l : loc).
+| HLPL_plus_loan (l : loan_id)
+| HLPL_plus_ptr (l : loan_id).
 
 Variant HLPL_plus_unit :=
-| HLPL_plus_borrow (l : loc)
-| HLPL_plus_loc (l : loc).
+| HLPL_plus_borrow (l : loan_id)
+| HLPL_plus_loc (l : loan_id).
 
 Variant HLPL_plus_bin := .
 
-Definition HLPL_plus_val := value HLPL_plus_zero HLPL_plus_unit HLPL_plus_bin.
+Notation HLPL_plus_val := (value HLPL_plus_zero HLPL_plus_unit HLPL_plus_bin).
 
 Variant HLPL_plus_binder :=
 | Var (v : var)
@@ -24,7 +26,7 @@ Variant HLPL_plus_binder :=
 Program Global Instance EqDec_binder : EqDec HLPL_plus_binder.
 Next Obligation. repeat decide equality. Qed.
 
-Definition HLPL_plus_state := state HLPL_plus_zero HLPL_plus_unit HLPL_plus_bin HLPL_plus_binder.
+Notation HLPL_plus_state := (state HLPL_plus_zero HLPL_plus_unit HLPL_plus_bin HLPL_plus_binder).
 
 Declare Scope hlpl_plus_scope.
 Delimit Scope hlpl_plus_scope with hlpl_plus.
@@ -48,7 +50,278 @@ Notation "'loc' l v" := (@vUnit HLPL_plus_zero HLPL_plus_unit HLPL_plus_bin (HLP
 (* Bind Scope hlpl_plus_scope with HLPL_plus_val. *)
 Open Scope hlpl_plus_scope.
 
-(* TODO: add a permission parameter. *)
-Inductive eval_path : HLPL_plus_state -> path -> permission -> spath -> spath -> Prop :=
-| Eval_nil s perm pi : eval_path s nil perm pi pi
-| Eval_deref_borrow_mut s p q : eval_path s (Deref :: p) Mut p (0 :: q)
+
+Global Instance Inhabited_HLPL_plus_val : Inhabited HLPL_plus_val := { default := bot }.
+
+(*
+Variant eval_proj (S : HLPL_plus_state) perm : proj -> spath -> spath -> Prop :=
+| Eval_Deref_MutBorrow q l v
+    (imm_or_mut : perm <> Mov)
+    (extract_q : S{{q}} = vUnit (HLPL_plus_borrow l) v) :
+    eval_proj S perm Deref q (q +++ [0])
+| Eval_Deref_Ptr_Locs q q' l w (imm_or_mut : perm <> Mov) :
+    S{{q}} = vZero (HLPL_plus_ptr l) -> valid_spath S q' -> S{{q'}} = vUnit (HLPL_plus_loc l) w ->
+    eval_proj S perm Deref q q'.
+
+(* TODO: name *)
+Variant eval_path_epsilon (S : HLPL_plus_state) perm : spath -> spath -> Prop :=
+| Eval_Loc q l v (imm_or_mut : perm <> Mov) (extract_q : S{{q}} = vUnit (HLPL_plus_loc l) v) :
+    eval_path_epsilon S perm q (q +++ [0]).
+*)
+
+(* TODO: eval_path represents a computation, that evaluates and accumulate the result over [...] *)
+Inductive eval_path (s : HLPL_plus_state) : path -> permission -> spath -> spath -> Prop :=
+(* Corresponds to R-Base and W-Base in the paper. *)
+| Eval_nil perm pi : eval_path s [] perm pi pi
+(* Coresponds to R-Deref-MutBorrow and W-Deref-MutBorrow in the paper. *)
+| Eval_Deref_MutBorrow p q l v r
+    (extract_q : s{{q}} = vUnit (HLPL_plus_borrow l) v)
+    (eval_q : eval_path s p Mut (q +++ [0]) r) :
+    eval_path s (Deref :: p) Mut q r
+| Eval_Deref_Ptr_Locs p q q' l w r :
+    s{{q}} = vZero (HLPL_plus_ptr l) -> valid_spath s q' -> s{{q'}} = vUnit (HLPL_plus_loc l) w ->
+    eval_path s p Mut q' r ->
+    eval_path s (Deref :: p) Mut q r
+| Eval_Loc proj P q r l v (extract_q : s{{q}} = vUnit (HLPL_plus_loc l) v) :
+    eval_path s (proj :: P) Mut (q +++ [0]) r -> eval_path s (proj :: P) Mut q r.
+Print eval_path.
+
+Lemma eval_path_valid (s : HLPL_plus_state) p perm q r
+  (valid_q : valid_spath s q) (eval_q_r : eval_path s p perm q r) :
+  valid_spath s r.
+Proof.
+  induction eval_q_r.
+  - assumption.
+  - apply IHeval_q_r. rewrite valid_spath_app. split; try assumption. rewrite extract_q.
+    constructor. constructor.
+  - auto.
+  - apply IHeval_q_r. rewrite valid_spath_app. split; try assumption. rewrite extract_q.
+    constructor. constructor.
+Qed.
+
+(*
+Definition eval_place (s : HLPL_plus_state) (p : place) (perm : permission) (r : spath) :=
+  exists i, find_index s (Var (fst p)) = Some i /\ eval_path s (snd p) perm (i, []) r.
+*)
+Notation eval_place s p perm r :=
+  (exists i, find_index s (Var (fst p)) = Some i /\ eval_path s (snd p) perm (i, []) r).
+
+Lemma eval_place_valid s p perm r (H : eval_place s p perm r) : valid_spath s r.
+Proof.
+  destruct H as (? & ? & ?). eapply eval_path_valid; try eassumption.
+  eapply find_index_valid_spath. eassumption.
+Qed.
+
+(* Setting up the definitions for judgements like "loan \notin v" or
+   "l is fresh". *)
+Definition state_contains (H : HLPL_plus_val -> Prop) (s : HLPL_plus_state) :=
+  exists p, valid_spath s p /\ H (s{{p}}).
+
+Definition value_contains (H : HLPL_plus_val -> Prop) (v : HLPL_plus_val) :=
+  exists p, valid_vpath v p /\ H (v{{p}}).
+
+Definition is_loan (v : HLPL_plus_val) :=
+  exists l, v = vZero (HLPL_plus_loan l).
+Definition contains_loan := value_contains is_loan.
+
+Definition is_mut_borrow (v : HLPL_plus_val) := exists l w, v = vUnit (HLPL_plus_borrow l) w.
+
+Definition contains_outer_loan v :=
+  exists l p, v{{p}} = vZero (HLPL_plus_loan l) /\ (forall q, vprefix q p -> ~is_mut_borrow (v{{q}})).
+
+Definition contains_outer_loc (v : HLPL_plus_val) :=
+  exists l w p, v{{p}} = vUnit (HLPL_plus_loc l) w /\ (forall q, vprefix q p -> ~is_mut_borrow (v{{q}})).
+
+Definition is_loc (v : HLPL_plus_val) :=
+  exists l w, v = vUnit (HLPL_plus_loc l) w.
+Definition contains_loc := value_contains is_loc.
+
+Variant is_loan_id (l : loan_id) : HLPL_plus_val -> Prop  :=
+| Is_loan_id_loan : is_loan_id l (vZero (HLPL_plus_loan l))
+| Is_loan_id_borrow w : is_loan_id l (vUnit (HLPL_plus_borrow l) w)
+| Is_loan_id_ptr : is_loan_id l (vZero (HLPL_plus_ptr l))
+| Is_loan_id_loc w : is_loan_id l (vUnit (HLPL_plus_loc l) w).
+
+(* TODO: rename "is_fresh" *)
+Definition is_fresh l s := ~state_contains (is_loan_id l) s.
+
+Definition is_borrow (v : HLPL_plus_val) :=
+  exists l w, v = vUnit (HLPL_plus_borrow l) w.
+
+Definition not_in_borrow (s : HLPL_plus_state) p :=
+  forall q, prefix q p /\ is_borrow (s{{q}}) -> q = p.
+
+Definition contains_bot (v : HLPL_plus_val) :=
+  value_contains (fun w => w = bot) v.
+
+Inductive copy_val : HLPL_plus_val -> HLPL_plus_val -> Prop :=
+| Copy_val_int (n : nat) : copy_val (vZero (HLPL_plus_int n)) (vZero (HLPL_plus_int n))
+| Copy_ptr l : copy_val (vZero (HLPL_plus_ptr l)) (vZero (HLPL_plus_ptr l))
+| Copy_loc l v w : copy_val v w -> copy_val (vUnit (HLPL_plus_loc l) v) w.
+
+Variant eval_op : HLPL_plus_state -> operand -> HLPL_plus_val -> HLPL_plus_state -> Prop :=
+| Eval_IntConst s n : eval_op s (IntConst n) (vZero (HLPL_plus_int n)) s
+(* TODO: place should be read in Imm mode. *)
+| Eval_copy s (p : place) q v : eval_place s p Mut q -> copy_val (s{{q}}) v ->
+    eval_op s (Copy p) v s
+| Eval_move s (p : place) q : eval_place s p Mov q -> ~contains_loan (s{{q}}) -> ~contains_bot (s{{q}}) ->
+    eval_op s (Move p) (s{{q}}) (s{{q <- bot}}).
+
+Variant eval_rvalue : HLPL_plus_state -> rvalue -> HLPL_plus_val -> HLPL_plus_state -> Prop :=
+| Eval_just s op v s' : eval_op s op v s' -> eval_rvalue s (Just op) v s'
+(* For the moment, the only operation is the natural sum. *)
+| Eval_bin_op s s' s'' op_l op_r m n : eval_op s op_l (vZero (HLPL_plus_int m)) s' ->
+   eval_op s' op_r (vZero (HLPL_plus_int n)) s'' ->
+   eval_rvalue s (BinOp op_l op_r) (vZero (HLPL_plus_int (m + n))) s''
+| Eval_pointer_loc s p q l v : eval_place s p Mut q -> s{{q}} = vUnit (HLPL_plus_loc l) v ->
+    ~contains_loan v -> ~contains_bot v ->
+    eval_rvalue s (&mut p) (vZero (HLPL_plus_ptr l)) s
+| Eval_pointer s p q l : eval_place s p Mut q -> ~contains_loan (s{{q}}) -> ~contains_bot (s{{q}}) ->
+    is_fresh l s -> ~is_loc (s{{q}}) ->
+    eval_rvalue s (&mut p) (vZero (HLPL_plus_ptr l)) (s{{q <- vUnit (HLPL_plus_loc l) (s{{q}})}}).
+Print eval_rvalue.
+
+Inductive reorg : HLPL_plus_state -> HLPL_plus_state -> Prop :=
+| Reorg_refl s : reorg s s
+| Reorg_trans s0 s1 s2 : reorg s0 s1 -> reorg s1 s2 -> reorg s0 s2
+| Reorg_end_borrow_m s (p q : spath) l v : valid_spath s p -> valid_spath s q ->
+    s{{p}} = (vZero (HLPL_plus_loan l)) -> s{{q}} = (vUnit (HLPL_plus_borrow l) v) ->
+    ~contains_loan v -> not_in_borrow s q ->
+    reorg s (s{{p <- v}}{{q <- bot}}).
+Print reorg.
+
+(* When introducing non-terminating features (loops or recursivity), the signature of the relation
+   is going to be:
+   HLPL_plus_state -> statement -> nat -> Option (statement_result * HLPL_plus_state) -> Prop
+*)
+Inductive eval_stmt : HLPL_plus_state -> statement -> statement_result -> HLPL_plus_state -> Prop :=
+| Eval_nop s : eval_stmt s Nop rUnit s
+| Eval_seq_unit S0 S1 S2 stmt_l stmt_r r (eval_stmt_l : eval_stmt S0 stmt_l rUnit S1)
+    (eval_stmt_r : eval_stmt S1 stmt_r r S2) : eval_stmt S0 (stmt_l ;; stmt_r) r S2
+| Eval_seq_panic S0 S1 stmt_l stmt_r (eval_stmt_l : eval_stmt S0 stmt_l rPanic S1) :
+    eval_stmt S0 (stmt_l ;; stmt_r) rPanic S1
+| Eval_assign S S' p rv v sp : eval_rvalue S rv v S' -> eval_place S' p Mut sp ->
+    ~contains_outer_loc (S'{{sp}}) -> ~contains_outer_loan (S'{{sp}}) ->
+    eval_stmt S (ASSIGN p <- rv) rUnit ((Anon, S'{{sp}}) :: S'{{sp <- v}}).
+
+(* TODO: introduce well-formedness judgement. *)
+Variant le_state_base : HLPL_plus_state -> HLPL_plus_state -> Prop :=
+(*
+| Le_refl S : le_state S S
+| Le_trans S0 S1 S2 : le_state S0 S1 -> le_state S1 S2 -> le_state S0 S2
+*)
+| Le_MutBorrow_To_Ptr S l p q v : disj p q -> S{{p}} = vZero (HLPL_plus_loan l) ->
+    S{{q}} = vUnit (HLPL_plus_borrow l) v ->
+    le_state_base (S{{p <- vUnit (HLPL_plus_loc l) v}}{{q <- vZero (HLPL_plus_ptr l)}}) S.
+
+Inductive refl_trans_closure {A : Type} (R : A -> A -> Prop) : A -> A -> Prop :=
+| Cl_base x y : R x y -> refl_trans_closure R x y
+| Cl_refl x : refl_trans_closure R x x
+| Cl_trans x y z : refl_trans_closure R x y -> refl_trans_closure R y z -> refl_trans_closure R x z.
+
+Definition le_state := refl_trans_closure le_state_base.
+
+Section MutBorrow_to_Ptr.
+  Context (S_r : HLPL_plus_state).
+  Context (l : loan_id).
+  Context (v : HLPL_plus_val).
+  Context (sp_loan sp_borrow : spath).
+  Context (valid_sp_loan : valid_spath S_r sp_loan).
+  Context (valid_sp_borrow : valid_spath S_r sp_borrow).
+  Context (Hdisj : disj sp_loan sp_borrow).
+  Context (HS_r_loan : S_r{{sp_loan}} = vZero (HLPL_plus_loan l)).
+  Context (HS_r_borrow : S_r{{sp_borrow}} = vUnit (HLPL_plus_borrow l) v).
+  Notation S_l := (S_r{{sp_loan <- vUnit (HLPL_plus_loc l) v}}{{sp_borrow <- vZero (HLPL_plus_ptr l)}}).
+
+  Notation "sp_l ~ sp_r" :=
+    ((sp_l = sp_r) \/
+     (exists vp_tail, sp_l = sp_loan +++ [0] ++ vp_tail /\ sp_r = sp_borrow +++ [0] ++ vp_tail))
+  (at level 1).
+
+  Lemma rel_prefix_sp_borrow sp_l sp_r (H : sp_l ~ sp_r)
+    (pref : strict_prefix sp_r sp_borrow) : sp_l = sp_r.
+  Proof.
+    destruct H as [ | H].
+    - assumption.
+    - exfalso. eapply strict_prefix_antisym.
+      + exact pref.
+      + destruct H as (vp_tail & _ & ?). exists 0, vp_tail. auto.
+  Qed.
+
+  Lemma rel_sp_borrow sp_l : sp_l ~ sp_borrow -> sp_l = sp_borrow.
+  Proof.
+    intros [? | H].
+    - assumption.
+    - exfalso. apply (strict_prefix_irrefl sp_borrow).
+      destruct H as (vp_tail & _ & ?). exists 0, vp_tail. auto.
+  Qed.
+
+  (* TODO: General property of paths *)
+  Lemma strict_prefix_sp_borrow q : strict_prefix q sp_borrow ->
+    strict_prefix q sp_loan \/ disj q sp_loan.
+  Admitted.
+
+  Lemma strict_prefix_sp_borrow_same_constructor q :
+    valid_spath S_r q -> strict_prefix q sp_borrow ->
+    same_constructor (S_l{{q}}) (S_r{{q}}).
+  Proof.
+    intros ? H. etransitivity.
+    - symmetry. apply same_constructor_subst_strict_prefix. admit. assumption.
+    - apply strict_prefix_sp_borrow in H. destruct H.
+      + symmetry. apply same_constructor_subst_strict_prefix; assumption.
+      + symmetry. apply same_constructor_subst_disj. assumption. assumption. symmetry. assumption.
+  Admitted.
+
+  (* TODO: only true for perm >= Mut, not for perm = Imm *)
+  Lemma eval_path_mut_borrow_to_ptr p sp_r sp_r' (H : eval_path S_r p Mut sp_r sp_r') :
+    valid_spath S_r sp_r -> forall sp_l, valid_spath S_l sp_l -> sp_l ~ sp_r ->
+      exists sp_l', sp_l' ~ sp_r' /\ eval_path S_l p Mut sp_l sp_l'.
+  Proof.
+    induction H as [ | | |]. Print eval_path. Check eval_path_ind.
+    - intros _ sp_l _ [ | (vp_tail & -> & ->)].
+      + exists sp_l. split; auto || constructor.
+      + eexists. split. right. exists vp_tail. split; reflexivity. constructor. 
+    - intros valid_sp_r sp_l valid_sp_l rel.
+      destruct (strict_comparable_spaths q sp_borrow) as [ Hprefix | | | ].
+      + apply rel_prefix_sp_borrow in rel; try assumption. rewrite rel.
+        assert (same_cons : same_constructor (S_l{{q}}) (S_r{{q}})).
+        { apply strict_prefix_sp_borrow_same_constructor. assumption. assumption. }
+        rewrite extract_q in same_cons.
+        destruct IHeval_path with (sp_l := q +++ [0]).
+        * admit. (* Validity argument, should be automatic. *)
+        * admit. (* Validity argument. *)
+        * auto.
+        * destruct H0. exists x. split; try assumption. eapply Eval_Deref_MutBorrow. admit. assumption.
+  Admitted.
+
+Lemma eval_place_mut_borrow_to_ptr p sp_r (H : eval_place S_r p Mut sp_r) :
+  exists sp_l, sp_l ~ sp_r /\ eval_place S_l p Mut sp_l.
+Proof.
+  destruct H as (i & ? & H).
+  apply eval_path_mut_borrow_to_ptr with (sp_l := (i, [])) in H.
+  - destruct H as (sp_l & ? & ?). exists sp_l. split; try assumption.
+    exists i. split. (* Need a lemma that says that substitution doesn't affect find_index. *)
+    admit. assumption.
+  - eapply find_index_valid_spath. eassumption.
+  - apply find_index_valid_spath with (b := Var (fst p)). admit. (* same. *)
+  - auto.
+Admitted.
+End MutBorrow_to_Ptr.
+
+(* TODO: simulation for eval_op *)
+Lemma eval_rvalue_sim S_l S_r S'_r rv v_r (Hle : le_state_base S_l S_r)
+  (Heval_rv : eval_rvalue S_r rv v_r S'_r) :
+  exists v_l S'_l, eval_rvalue S_l rv v_l S'_l /\ le_state ((Anon, v_l) :: S'_l) ((Anon, v_r) :: S'_r).
+Proof.
+  induction Heval_rv.
+  - admit. (* TODO: lemma for operands. *)
+  - admit. (* Same. *)
+  - destruct Hle as [S_r l' sp_loan sp_borrow].
+    eapply eval_place_mut_borrow_to_ptr with (sp_loan := sp_loan) (sp_borrow := sp_borrow) in H.
+    + admit.
+    + admit. (* missing validity condition. *)
+    + admit. (* same *)
+    + assumption.
+    + eassumption.
+    + eassumption.
+Admitted.
